\chapter{Vector Spaces}

%%% R^n and C^n {{{

\section{\texorpdfstring{$\R^{n}$}{R\^{}n} and \texorpdfstring{$\C^{n}$}{C\^{}n}}

\begin{exercise}{7}
	Show that for every \( \alpha \in \C \), there exists a unique \( \beta \in \C \)
	such that \( \alpha + \beta = 0 \).
\end{exercise}

\begin{proof}
	Suppose \( \alpha = a + bi \). Let \( \beta = -a - bi \). Then
	\[
		\alpha + \beta = (a - a) + (b - b)i = 0,
	\]
	proving existence.

	Suppose there exists \( \gamma \in \C \) such that \( \alpha + \gamma = 0 \). Then
	\[
		\gamma = \gamma + (\alpha + \beta) = (\gamma + \alpha) + \beta = \beta,
	\]
	proving uniqueness.
\end{proof}

%%% }}}

%%% Definition of Vector Space {{{

\section{Definition of Vector Space}

\begin{exercise}{6}
	Let \( \infty \) and \( -\infty \) denote two distinct objects, neither of
	which is in \( \R \). Define an addition and scalar multiplication on
	\( \R \cup \{\infty\} \cup \{-\infty\} \) as you could guess from the notation.
	Specifically, the sum and product of two real numbers is as usual, and for
	\( t \in \R \) define
	\[
		t\infty = \begin{cases}
			-\infty & \text{if} \ t < 0, \\
			0       & \text{if} \ t = 0, \\
			\infty  & \text{if} \ t > 0,
		\end{cases} \quad
		t(-\infty) = \begin{cases}
			\infty  & \text{if} \ t < 0, \\
			0       & \text{if} \ t = 0, \\
			-\infty & \text{if} \ t > 0,
		\end{cases} \\
		t + \infty = \infty + t = 
	\]
	Is \( \R \cup \{\infty\} \cup \{-\infty\} \) a vector space over \( \R \)? Explain.
\end{exercise}

%%% }}}

%%% Subspaces {{{

\section{Subspaces}

\begin{exercise}{12}
	Prove that the union of two subspaces of \( V \) is a subspace of \( V \) if
	and only if one of the subspaces is contained in the other.
\end{exercise}

\begin{proof}
	Suppose \( U \) and \( W \) are subspaces of \( V \), such that \( U \cup W \)
	is also a subspace and neither is contained in the other.
	In other words, \( U \not\subset W \) and \( W \not\subset U \).
	Let \( u \in U - W \) and \( w \in W - U \).
	Since \( U \cup W \) is a subspace of \( V \), we have \( u + w \in U \cup W \).
	However,
	\begin{align*}
		u + w \in U &\Rightarrow w = (u + w) - u \in U, \\
		u + w \in W &\Rightarrow u = (u + w) - w \in W,
	\end{align*}
	which implies that \( u + w \) is in neither \( U \) nor \( W \), a contradiction.
\end{proof}

%%% }}}
